TypeSystem.v
@@ -11,12 +11,14 @@ Inductive has_type : context -> term -> ty -> Prop :=
   | T_Abs : forall ctx x t2 T1 T2, 
         has_type (extend ctx x T1) t2 T2 ->
         has_type ctx (tm_abs x T1 t2) (arrow T1 T2 Trust)
-  | T_App : forall ctx t1 t2 T11 T12 s, 
+  | T_App : forall ctx t1 t2 T11 T11' T12 s u, 
         has_type ctx t1 (arrow T11 T12 s) -> 
-        has_type ctx t2 T12 ->
-        has_type ctx (tm_app t1 t2) (update_secty T12 s)
-  | T_If : forall ctx t1 t2 t3 T,
-        has_type ctx t1 BoolT ->
+        has_type ctx t2 T11' ->
+        subtype T11' T11     ->
+        u = update_secty T12 s -> 
+        has_type ctx (tm_app t1 t2) u
+  | T_If : forall ctx t1 t2 t3 T s,
+        has_type ctx t1 (ty_bool s) ->
         has_type ctx t2 T     ->
         has_type ctx t3 T     -> 
         has_type ctx (tm_if t1 t2 t3) T
@@ -41,6 +43,8 @@ Tactic Notation "has_type_cases" tactic(first) ident(c) :=
            Case_aux c "T_Trust" | Case_aux c "T_Untrust" | Case_aux c "T_Check" |
            Case_aux c "T_Sub"].
 
+Hint Constructors has_type.
+
 (** inversion lemmas for subtyping **)
 
 Lemma sub_inversion_base : 
@@ -62,6 +66,8 @@ Proof.
   induction Hsub ; try solve by inversion ; try intros ; try (inv HeqV).
   repeat eexists ; repeat split ; eauto.
 Qed.
+
+Hint Resolve sub_inversion_base sub_inversion_arrow.
 
 (** canonical forms lemmas **)
 
@@ -119,9 +125,9 @@ Proof with eauto.
           as [x [S1 [s2 Heq]]] ... subst.
         exists (subst x t2 s2) ...
       SSCase "t2 can step".
-        destruct H0 as [t2' Ht'] ; exists (tm_app t1 t2') ...
+         destruct H1 as [t2' Ht'] ; exists (tm_app t1 t2') ...
     SCase "t1 can step".
-      destruct H as [t1' Ht1'].
+      destruct H0 as [t1' Ht1'].
       exists (tm_app t1' t2) ...
   Case "T_If".
     destruct IHHty1 ...
@@ -160,4 +166,214 @@ Proof with eauto.
     exists T2 ; exists Trust ; split ...   
   Case "T_Sub".
     destruct IHhas_type as [S2 [s' [H1 H2]]] ...
+Qed.
+
+Lemma typing_inversion_var : 
+  forall ctx x T, has_type ctx (tm_var x) T ->
+    exists S, ctx x = Some S /\ subtype S T.
+Proof with eauto.
+  intros ctx x T Hty.
+  remember (tm_var x) as V.
+  has_type_cases(induction Hty) Case ; intros ; inv HeqV ; try solve by inversion.
+  Case "T_Var".
+    repeat eexists ...
+  Case "T_Sub".
+    destruct IHHty ...
+    exists x0.    
+    destruct H0.
+    split ...
+Qed.
+
+Lemma typing_inversion_true : 
+  forall ctx T, has_type ctx tm_true T ->
+    subtype (ty_bool Trust) T.
+Proof with eauto.
+  intros ctx T Hty.
+  remember tm_true as t.
+  has_type_cases (induction Hty) Case ; inv Heqt...
+Qed.
+
+Lemma typing_inversion_false :
+  forall ctx T, has_type ctx tm_false T ->
+    subtype (ty_bool Trust) T.
+Proof with eauto.
+  intros ctx T Hty.
+  remember tm_false as t.
+  has_type_cases (induction Hty) Case ; inv Heqt ...
+Qed.
+
+Lemma typing_inversion_app :
+  forall ctx t1 t2 T2, has_type ctx (tm_app t1 t2) T2 ->
+    exists T1, exists s, has_type ctx t1 (arrow T1 T2 s) /\ has_type ctx t2 T1.
+Proof with eauto.
+  intros ctx t1 t2 T2 Hty.
+  remember (tm_app t1 t2) as t.
+  has_type_cases (induction Hty) Case ; intros ; inv Heqt ; try solve by inversion ...
+  Case "T_App".
+    repeat eexists ...
+  Case "T_Sub".
+    destruct IHHty ...
+    destruct H0 as [s [H1 H2]].
+    repeat eexists ...   
+Qed.
+
+Lemma typing_inversion_trust : 
+  forall ctx t T, has_type ctx (tm_trust t) T ->
+    exists T', has_type ctx t T' /\ subtype T' T.
+Proof with eauto.
+   intros ctx t T Hty.
+   remember (tm_trust t) as V.
+   has_type_cases (induction Hty) Case ; inv HeqV ; try solve by inversion ...
+   Case "T_Sub".
+     destruct IHHty ...
+     destruct H0 as [H1 H2].
+     eexists ; split ...
+Qed.
+
+Lemma typing_inversion_distrust :
+  forall ctx t T, has_type ctx (tm_distrust t) T ->
+    exists T', has_type ctx t T' /\ subtype T' T.
+Proof with eauto.
+  intros ctx t T Hty.
+  remember (tm_distrust t) as V.
+  has_type_cases (induction Hty) Case ; inv HeqV ; try solve by inversion ...
+  Case "T_Sub".
+    destruct IHHty ...
+    destruct H0 as [H1 H2].
+    eexists ; split ...
+Qed.
+
+Lemma typing_inversion_check : 
+  forall ctx t T, has_type ctx (tm_check t) T ->
+    exists T', has_type ctx t T' /\ subtype T' T.
+Proof with eauto.
+  intros ctx t T Hty.
+  remember (tm_check t) as V.
+  has_type_cases (induction Hty) Case ; inv HeqV ; try solve by inversion.
+  Case "T_Check".
+    eexists ; split ...
+  Case "T_Sub".
+    eexists ; split ...
+    destruct IHHty as [ty [H1 H2]]...
+Qed.
+
+Lemma typing_inversion_if :
+  forall ctx t1 t2 t3 T, has_type ctx (tm_if t1 t2 t3) T ->
+    exists s, has_type ctx t1 (ty_bool s) /\ has_type ctx t2 T /\ has_type ctx t3 T.
+Proof with eauto.
+  intros ctx t1 t2 t3 T Hty.
+  remember (tm_if t1 t2 t3) as V.
+  has_type_cases (induction Hty) Case ; inv HeqV ; try solve by inversion ...
+  Case "T_Sub".
+    destruct IHHty as [s [H1 [H2 H3]]] ...
+    eexists ; repeat split ...
+Qed.
+
+(** context invariance **)
+
+Inductive appears_free_in : id -> term -> Prop :=
+  | afi_var : forall i, appears_free_in i (tm_var i)
+  | afi_app1 : forall i t1 t2, appears_free_in i t1 ->
+                               appears_free_in i (tm_app t1 t2)
+  | afi_app2 : forall i t1 t2, appears_free_in i t2 ->
+                               appears_free_in i (tm_app t1 t2)
+  | afi_abs : forall i x T t, i <> x -> appears_free_in i t ->
+                              appears_free_in i (tm_abs x T t)
+  | afi_if1 : forall i t1 t2 t3, appears_free_in i t1 ->
+                                 appears_free_in i (tm_if t1 t2 t3)
+  | afi_if2 : forall i t1 t2 t3, appears_free_in i t2 ->
+                                 appears_free_in i (tm_if t1 t2 t3)
+  | afi_if3 : forall i t1 t2 t3, appears_free_in i t3 ->
+                                 appears_free_in i (tm_if t1 t2 t3)
+  | afi_trust : forall i t, appears_free_in i t ->
+                            appears_free_in i (tm_trust t)
+  | afi_distrust : forall i t, appears_free_in i t ->
+                               appears_free_in i (tm_distrust t)
+  | afi_check : forall i t, appears_free_in i t ->
+                            appears_free_in i (tm_check t).
+
+Hint Constructors appears_free_in.
+  
+Lemma context_invariance :
+  forall ctx ctx' t S, has_type ctx t S ->
+    (forall x, appears_free_in x t -> ctx x = ctx' x) ->
+    has_type ctx' t S.
+Proof with eauto.
+  intros. generalize dependent ctx'.
+  has_type_cases (induction H) Case ; intros ctx' Heqv ; try solve by inversion ...
+  Case "T_Var".
+    apply T_Var. rewrite <- Heqv...
+  Case "T_Abs".
+    apply T_Abs ...
+    apply IHhas_type. intros x0 Hafi ; unfold extend.
+    remember (beq_id x x0) as e ; destruct e ...
+    symmetry in Heqe.
+    apply beq_id_false_not_eq in Heqe ...
+  Case "T_App".
+    eapply T_App ...
+  Case "T_If".
+    eapply T_If ...
+Qed.
+
+Lemma free_in_context :
+  forall i ctx t T,
+    appears_free_in i t ->
+    has_type ctx t T ->
+    exists T', ctx i = Some T'.
+Proof with eauto.
+  intros i ctx t T Hafi Hty.
+  has_type_cases (induction Hty) Case ; inv Hafi ...
+  Case "T_Abs".
+    destruct (IHHty H4) as [T Ht]. exists T. unfold extend in Ht.
+    apply not_eq_beq_id_false in H2. rewrite beq_id_sym in H2.
+    rewrite H2 in Ht ...
+Qed.
+
+(** substitution lemma **)
+
+Hint Resolve typing_inversion_false typing_inversion_true.
+
+Lemma substitution_preserves_typing : 
+  forall ctx i T v t T',
+    has_type (extend ctx i T) t T' ->
+    has_type empty v T ->
+    has_type ctx (subst i v t) T'.
+Proof with eauto.
+  intros ctx i T v t T' Hty' Htyv.
+  generalize dependent T'. generalize dependent ctx.
+  term_cases (induction t) Case ; intros ; simpl  ...
+  Case "tm_if".
+    apply typing_inversion_if in Hty'.
+    destruct Hty' as [s [H1 [H2 H3]]].
+    apply IHt1 in H1.
+    apply IHt2 in H2.
+    apply IHt3 in H3.
+    eapply T_If ...
+  Case "tm_var".
+    rename i into y.
+    apply typing_inversion_var in Hty'.
+    destruct Hty' as [S [H1 H2]].
+    unfold extend in *. 
+    remember (beq_id y i0) as e ; destruct e.
+    SCase "i = i0".
+      apply beq_id_eq in Heqe. subst. inv H1.
+    apply T_Sub with S.
+    apply context_invariance with empty ... intros x contra.
+    destruct (free_in_context _ empty _ S contra) as [T1 HT1]... 
+    inv HT1. auto. eapply T_Sub ...
+  Case "tm_app".
+    destruct (typing_inversion_app _ _ _ _ Hty') as [S [s [Hty1 Hty2]]] ...
+    eapply T_App ...
+
+(** preservation **)
+
+Theorem preservation : 
+  forall t t' T, has_type empty t T ->
+    t ==> t' -> has_type empty t' T.
+Proof with eauto.
+ intros t t' T HT.
+ remember (@empty ty) as ctx. generalize dependent Heqctx.
+ generalize dependent t'.
+ has_type_cases (induction HT) Case ; intros t' Heqctx HE ; try solve by inversion...
+ inv HE ...
 Qed.
